# Direct Proofs

## If P, then Q

**Proposition:** If P is true, then Q is true.

*We are asserting the truth of the implication $P\implies Q$.
If $P$ is false, then the implication is automatically true.
So from a practical point of view, we must show that
whenver $P$ is true, $Q$ is also true.*


**Proof:** Suppose P.

(bunch of stuff)

Therefore Q.

## Simple example

**Proposition:** The sum of two odd integers is even.


##

**Proposition:** The sum of two odd integers is even.

**Proof:**

Suppose $a$ and $b$ are odd integers.

\vfill

Therefore $a+b$ is even.

##

**Proposition:** The sum of two odd integers is even.

**Proof:**

Suppose $a$ and $b$ are odd integers.

Then there are integers $k$ and $u$ so that $a=2k+1$ and $b=2u+1$.

\vfill 

Therefore $a+b$ is even.

##

**Proposition:** The sum of two odd integers is even.

**Proof:**

Suppose $a$ and $b$ are odd integers.

Then there are integers $k$ and $u$ so that $a=2k+1$ and $b=2u+1$.

Therefore
$$a+b=(2k+1)+(2u+1)=2(k+u)+2=2(k+u+1)$$

\vfill
Therefore $a+b$ is even.

##

**Proposition:** The sum of two odd integers is even.

**Proof:**

Suppose $a$ and $b$ are odd integers.

Then there are integers $k$ and $u$ so that $a=2k+1$ and $b=2u+1$.

Therefore $a+b=(2k+1)+(2u+1)=2(k+u)+2=2(k+u+1)$

The definition of even integer says that an integer $x$ is even if there is an integer
$y$ so that $x=2y$.   We found that $a+b = 2(k+u+1)$ where $k+u+1$ is an integer.

\vfill

Therefore $a+b$ is even.
