# Fibonacci numbers

## Fibonacci Numbers

![Fibonacci](../../png/fibonacci.jpg){width=2in}

The Fibonacci numbers $F_n$ are defined by a *recursive* formula.  The first two numbers
are given by $F_1=1$ and $F_2=1$ and, for all $n\ge 3$, $F_n=F_{n-1}+F_{n-2}$.

$$1,1,2,3,5,8,13,21,34,55,89,...$$

## Fibonacci Numbers and the Golden Ratio

See [Donald Duck in Mathmagic Land](https://youtu.be/U_ZHsk0-eF0) (7 minute mark - 14 minute mark).

## Fibonacci Numbers and the Golden Ratio

The golden ratio 
$$
\phi=\frac{1+\sqrt{5}}{2}
$$
is the larger root of the quadratic polynomial $x^2-x-1=0$.

**Proposition:** The ratio of successive Fibonacci numbers $F_{n+1}/F_{n}$ converges to the Golden ratio.

## Some Data 

```
1		1		1.000000000
1		2		2.000000000
2		3		1.500000000
3		5		1.666666667
5		8		1.600000000
8		13		1.625000000
13		21		1.615384615
21		34		1.619047619
34		55		1.617647059
55		89		1.618181818
89		144		1.617977528
144		233		1.618055556
233		377		1.618025751
377		610		1.618037135
610	 	987		1.618032787
```

## Fibonacci Numbers cont'd

**Proposition:** $F_{n+1}^2-F_{n}F_{n+1}-F_{n}^2=(-1)^{n}$.

\begin{align*}
3^2-(2)(3)-2^2&=-1 \\
5^2-(3)(5)-3^2&=1 \\
8^2-(5)(8)-5^2&=-1 \\
\end{align*}

**Corollary:** $\lim_{n\to\infty}\frac{F_{n+1}}{F_{n}}=\phi$.

**Proof:** Divide through by $F_{n}^2$:

$$
(\frac{F_{n+1}}{F_{n}})^2-(\frac{F_{n+1}}{F_{n}})-1=\frac{(-1)^{n}}{F_{n}^2}
$$

The right hand side goes to zero, so $(F_{n+1}/F_{n})$ converges to a root of the polynomial which
is greater than one.

## Proof of proposition

First check that $F_{2}^2-F_{1}F_{2}-F_{1}^2=-1$, which is $1^2-1-1=-1$ as we want.

- Now suppose that the formula holds for $F_{n}$, so $F_{n}^2-F_{n}F_{n-1}-F_{n-1}^2=(-1)^{n-1}$.
- Consider $F_{n+1}^2-F_{n+1}F_{n}-F_{n}^2$. 
- Substitute $F_{n+1}=F_{n}+F_{n-1}$ to get

\begin{multline*}
(F_{n}+F_{n-1})^2-(F_{n}+F_{n-1})F_{n}-F_{n}^2 = \\ F_{n}^2+2F_{n}F_{n-1}+F_{n-1}^2-F_{n}^2-F_{n-1}F_{n}-F_{n}^2 
\end{multline*}

Then the right hand side of this equation is 

$$
-F_{n}^2+F_{n}F_{n-1}+F_{n-1}^2= -(F_{n}^2-F_{n}F_{n-1}-F_{n-1}^2) =(-1)^{n}
$$

where we used the inductive hypothesis to in the second-to-last step.

